vale/code/arch/x64/X64.Stack_Sems.fst
@@ -1,0 +1,4 @@
+module X64.Stack_Sems
+
+let stack_to_s s = admit()
+let stack_from_s s = admit()
