vale/code/arch/x64/X64.Stack_Sems.fsti
@@ -1,0 +1,12 @@
+module X64.Stack_Sems
+
+open X64.Machine_s
+open X64.Stack_i
+module S = X64.Bytes_Semantics_s
+
+val stack_to_s: (s:stack) -> Tot S.stack
+val stack_from_s: (s:S.stack) -> Tot stack
+
+val lemma_state_of_to (s:stack) : Lemma 
+  (stack_from_s (stack_to_s s) == s)
+  [SMTPat (stack_from_s (stack_to_s s))]
