vale/code/arch/x64/X64.Stack_i.fst
@@ -1,0 +1,8 @@
+module X64.Stack_i
+
+let stack = admit()
+
+let valid_src_stack64 i st = admit()
+let valid_dst_stack64 i st = admit()
+let load_stack64 i st = admit()
+let store_stack64 i v h = admit()
