vale/code/arch/x64/X64.Stack_i.fsti
@@ -1,0 +1,10 @@
+module X64.Stack_i
+
+open X64.Machine_s
+
+val stack: Type u#1
+
+val valid_src_stack64 : ptr:int -> h:stack -> GTot bool
+val valid_dst_stack64 : ptr:int -> h:stack -> GTot bool
+val load_stack64 : ptr:int -> h:stack -> GTot nat64
+val store_stack64 : ptr:int -> v:nat64 -> h:stack -> GTot stack
